Semantic/Stlc.lean
@@ -1,1 +1,17 @@
+/- Syntax -/
 import Semantic.Stlc.Syntax
+
+/- Substitution -/
+import Semantic.Stlc.Substitution
+
+/- Big-step operational semantics -/
+import Semantic.Stlc.BigStep
+
+/- Denotation of types -/
+import Semantic.Stlc.Denotation
+
+/- Type system definition -/
+import Semantic.Stlc.TypeSystem
+
+/- Semantic type soundness -/
+import Semantic.Stlc.Soundness
