Semantic/Stlc/Soundness.lean
@@ -7,12 +7,41 @@ theorem eval_num_val {v : Exp 0}
   Eval v v := by
   induction hv <;> grind [Eval]
 
+theorem eval_num_val_eq
+  (hv : v.IsNumVal)
+  (hev : Eval v v') :
+  v = v' := by
+  induction hv generalizing v'
+  case nzero =>
+    cases hev; rfl
+  case nsucc _ ih =>
+    cases hev
+    aesop
+
+theorem eval_bool_val_eq
+  (hv : v.IsBoolVal)
+  (hev : Eval v v') :
+  v = v' := by
+  cases hv
+  case btrue =>
+    cases hev; rfl
+  case bfalse =>
+    cases hev; rfl
+
 theorem eval_val {v : Exp 0}
   (hv : v.IsVal) :
   Eval v v := by
   cases hv <;> try grind [Eval]
   case bool hv => cases hv <;> grind [Eval]
   case num hv => apply eval_num_val hv
+
+theorem eval_val_eq
+  (hv : v.IsVal)
+  (hev : Eval v v') :
+  v = v' := by
+  cases hv <;> try grind [Eval]
+  case bool hv => apply eval_bool_val_eq hv hev
+  case num hv => apply eval_num_val_eq hv hev
 
 theorem typed_store_lookup
   (hts : TypedStore s Γ)
@@ -54,13 +83,19 @@ theorem sem_typ_nsucc
   { simp [Ty.val_denot]
     grind [Exp.IsNumVal] }
 
+theorem abs_val_is_val
+  (hv : Exp.IsAbsVal v) :
+  v.IsVal := by
+  cases hv
+  grind [Exp.IsVal]
+
 theorem val_denot_is_val
   (hv : Ty.val_denot T v) :
   v.IsVal := by
   cases T
   case bool => simp [Ty.val_denot] at hv; grind [Exp.IsVal]
   case nat => simp [Ty.val_denot] at hv; grind [Exp.IsVal]
-  case arrow => simp [Ty.val_denot] at hv; exact hv.left
+  case arrow => simp [Ty.val_denot] at hv; apply abs_val_is_val hv.left
 
 theorem sem_typ_abs
   (ht : (Γ,x:T) ⊨ e : U) :
@@ -71,7 +106,7 @@ theorem sem_typ_abs
   constructor; constructor
   { apply eval_val; grind [Exp.IsVal] }
   { simp [Ty.val_denot]
-    constructor; try grind [Exp.IsVal]
+    constructor; try grind [Exp.IsAbsVal]
     intro arg harg
     unfold SemanticTyping at ht
     have hvarg := val_denot_is_val harg
@@ -81,15 +116,112 @@ theorem sem_typ_abs
       simp [TypedStore]
       aesop
     specialize ht s' hts'
-    sorry }
+    simp [Ty.exp_denot] at ht ⊢
+    have ⟨v0, hev0, hv0⟩ := ht
+    use v0
+    apply And.intro _ hv0
+    { apply Eval.ev_app
+      · apply eval_val; grind [Exp.IsVal]
+      · apply eval_val hvarg
+      · simp [Exp.subst_comp]
+        rw [Subst.fromStore_openVar_comp (hv := hvarg)]
+        exact hev0
+    }
+  }
+
+theorem sem_typ_app
+  (ht1 : Γ ⊨ e1 : Ty.arrow T U)
+  (ht2 : Γ ⊨ e2 : T) :
+  (Γ ⊨ .app e1 e2 : U) := by
+  intro s hts
+  specialize ht1 s hts
+  specialize ht2 s hts
+  simp only [Ty.exp_denot] at *
+  have ⟨vf, hevf, hvf⟩ := ht1
+  have ⟨va, heva, hva⟩ := ht2
+  simp [Ty.val_denot] at hvf
+  cases hvf.left
+  have := hvf.right va hva
+  simp [Ty.exp_denot] at this
+  have ⟨v, hev, vdenot⟩ := this
+  use v
+  apply And.intro _ vdenot
+  apply Eval.ev_app
+  { exact hevf }
+  { exact heva }
+  { cases hev
+    rename_i hev1 hev2 hev3
+    cases (eval_val_eq (by constructor) hev1)
+    cases (eval_val_eq (val_denot_is_val hva) hev2)
+    exact hev3 }
+
+theorem sem_typ_pred
+  (ht : Γ ⊨ e : Ty.nat) :
+  (Γ ⊨ .pred e : Ty.nat) := by
+  intro s hts
+  specialize ht s hts
+  simp only [Ty.exp_denot] at *
+  have ⟨v0, hev0, v0denot⟩ := ht
+  simp [Ty.val_denot] at v0denot
+  cases v0denot
+  case nzero =>
+    use .nzero
+    apply And.intro _ (by grind [Ty.val_denot, Exp.IsNumVal])
+    exact Eval.ev_pred_nzero hev0
+  case nsucc n0 hv =>
+    use n0
+    apply And.intro _ (by grind [Ty.val_denot, Exp.IsNumVal])
+    exact Eval.ev_pred_nsucc hev0 hv
+
+theorem sem_typ_iszero
+  (ht : Γ ⊨ e : Ty.nat) :
+  (Γ ⊨ .iszero e : Ty.bool) := by
+  intro s hts
+  specialize ht s hts
+  simp only [Ty.exp_denot] at *
+  have ⟨v0, hev0, v0denot⟩ := ht
+  simp [Ty.val_denot] at v0denot
+  cases v0denot
+  case nzero =>
+    use .btrue
+    apply And.intro _ (by grind [Ty.val_denot, Exp.IsBoolVal])
+    exact Eval.ev_iszero_nzero hev0
+  case nsucc n0 hv =>
+    use .bfalse
+    apply And.intro _ (by grind [Ty.val_denot, Exp.IsBoolVal])
+    exact Eval.ev_iszero_nsucc hev0 hv
+
+theorem sem_typ_cond
+  (ht1 : Γ ⊨ e1 : Ty.bool)
+  (ht2 : Γ ⊨ e2 : T)
+  (ht3 : Γ ⊨ e3 : T) :
+  (Γ ⊨ .cond e1 e2 e3 : T) := by
+  intro s hts
+  specialize ht1 s hts
+  specialize ht2 s hts
+  specialize ht3 s hts
+  simp only [Ty.exp_denot] at *
+  have ⟨v1, hev1, v1denot⟩ := ht1
+  have ⟨v2, hev2, v2denot⟩ := ht2
+  have ⟨v3, hev3, v3denot⟩ := ht3
+  simp [Ty.val_denot] at v1denot
+  cases v1denot
+  case btrue =>
+    use v2
+    apply And.intro _ v2denot
+    exact Eval.ev_cond_true hev1 hev2 hev3
+  case bfalse =>
+    use v3
+    apply And.intro _ v3denot
+    exact Eval.ev_cond_false hev1 hev2 hev3
 
 theorem soundness
   (ht : Γ ⊢ e : T) :
   (Γ ⊨ e : T) := by
-  induction ht
-  case var hb => apply sem_typ_var hb
-  case abs => sorry
-  case app => sorry
+  induction ht <;>
+    try (solve |
+      grind [sem_typ_var, sem_typ_abs, sem_typ_app, sem_typ_nsucc,
+        sem_typ_pred, sem_typ_iszero, sem_typ_cond])
   case btrue =>
     intro s hts
     simp [Ty.exp_denot]
@@ -111,7 +243,3 @@ theorem soundness
     split_ands
     { grind [Exp.subst, Eval] }
     { simp [Ty.val_denot]; grind [Exp.IsNumVal] }
-  case nsucc ih => apply sem_typ_nsucc ih
-  case pred => sorry
-  case iszero => sorry
-  case cond => sorry
